LeanSts/State.lean
@@ -6,11 +6,19 @@ import LeanSts.Testing
 def updateFn [DecidableEq α] (f : α → β) (a : α) (b : β) : α → β :=
   λ (x : α) => if x = a then b else f x
 
-notation st"[ " a " ↦ " b " ]" => updateFn st a b
+def updateFn2 [DecidableEq α] [DecidableEq β] (f : α → β → γ)  (a : α) (b : β) (c : γ) : α → β → γ :=
+  λ (x : α) (y : β) => if x = a && y = b then c else f x y
+
+notation f"[ " a " ↦ " b " ]" => updateFn f a b
+notation f"[ " a " , " b " ↦ " c " ]" => updateFn2 f a b c
 
 @[simp] lemma updateFn_unfold [DecidableEq α] (f : α → β) (a : α) (b : β) (x : α) :
   (f[a ↦ b]) x = if x = a then b else f x := by
   simp only [updateFn]
+
+@[simp] lemma updateFn2_unfold  [DecidableEq α] [DecidableEq β] (f : α → β → γ)  (a : α) (b : β) (c : γ) :
+  (f[a , b ↦ c]) x y = if x = a && y = b then c else f x y := by
+  simp only [updateFn2]
 
 -- TODO: write a macro to define SampleableExt instances for Structures
 -- See https://github.com/verse-lab/lean-sts/commit/228605e7bb54c9f7cfec5d437f79c9607fb413fa
